fix: internalize nested ground patterns when activating ematch theorems
This PR internalize nested ground patterns when activating ematch
theorems in the (WIP) `grind` tactic.

tests/lean/run/grind_pattern2.lean
@@ -37,3 +37,37 @@ example [DecidableEq α] (s₁ s₂ : Set α) (a₁ a₂ : α) :
         ¬ contains s₂ a₂ → s₂ = insertElem s₁ a₁ → a₁ = a₂ → False := by
   fail_if_success grind
   sorry
+
+def a := 10
+def b := 20
+def foo (x : List Nat) (y : List Nat) := x ++ y ++ x
+
+theorem fooThm : foo x [a, b] = x ++ [a, b] ++ x := rfl
+
+/--
+info: [grind.pattern] fooThm: [foo #0 `[[a, b]]]
+-/
+#guard_msgs in
+grind_pattern fooThm => foo x [a, b]
+
+
+/--
+warning: declaration uses 'sorry'
+---
+info: [grind.internalize] foo x y
+[grind.pattern] activated `fooThm`
+[grind.internalize] [a, b]
+[grind.internalize] Nat
+[grind.internalize] a
+[grind.internalize] [b]
+[grind.internalize] b
+[grind.internalize] []
+[grind.internalize] x
+[grind.internalize] y
+[grind.internalize] z
+-/
+#guard_msgs in
+set_option trace.grind.internalize true in
+example : foo x y = z → False := by
+  fail_if_success grind
+  sorry
